#### Hilbert-Style Proof System

> [!NOTE]
>
> We know that every proof system has language part and the inference part, so this time we will develop everything in this structure.

**Language Part**

1. Alphabet

   $\Sigma = \{(,),\neg,\rightarrow,p,q,r,...\}$

2. Formula

   - Atoms p, q, r, ... are formulas.
   - If A and B are formulas, then($\neg A$), ($A\rightarrow B$) are also formulas.
   - Only expressions of $\Sigma$ that are generated by 1 and 2 are formulas.

**Inference Part**

1. Axioms

   - A~1~: $A\rightarrow (B \rightarrow A)$
   - A~2~: $(A\rightarrow (B\rightarrow C))\rightarrow((A\rightarrow B)\rightarrow(A\rightarrow C))$
   - A~3~: $(\neg A\rightarrow \neg B)\rightarrow (B \rightarrow A)$

2. Inference Rule

   - Modus Ponens

     > 1. $A\rightarrow B$
     > 2. $A$
     > 3. $B$ (According to the Modus Ponens)
     >
     > > [!NOTE]
     > >
     > > Notation Form:
     > >
     > > $r_{mp}=\frac{A,A\rightarrow B}{B}$

3. Another Definition
   - If $A$ $\in$ $\Sigma$, then $\Sigma \vdash A$.

**Formation of the Proof**

1. A formal proof is a logical chain from the assumptions to the conclusions.

2. The chain has to be finite.

3. Each link in the chain might be 

   - Axioms
   - Premises
   - Intermediate conclusion by the inference rules, for example, in the Hilbert system we will find that there is only one kind of the inference rule, called the Modus Ponens.

4. If we want to prove the statement A is correct in the Hilbert System, the appearance of the formula sequence should be like 

   - A~1~

   - A~2~

   - A~3~

   - ...

   - A

     Then we can just prove the statement A in a proper form.

5. Formation

   > If a formula A has a proof with premises $\Sigma$, then we say that "A can be proved from $\Sigma$".
   >
   > It will be denoted as $\Sigma \vdash_{H} A$, or you can just simplify it as $\Sigma\vdash A$, but here I prefer to write with the notation of H, because it tells that it is just a conclusion from the premises by the rule in the Hilbert System.
   >
   > **But I think the notation below is the most important!**
   >
   > > [!IMPORTANT]
   > >
   > > If $\Sigma = \varnothing$, then we can denote the former expression as $\vdash A$, which means that **A is now a theorem in the Hilbert System.**
   >
   > **And There is also another useful trick!**
   >
   > > [!IMPORTANT]
   > >
   > > If $A\in \Sigma$, then $\Sigma \vdash A$.

**Proof in the Hilbert System**

Example One:

> We need you to prove $\vdash A \rightarrow A$ in the Hilbert system.

Solution:

> $$
> \begin{aligned}
> &\vdash A\rightarrow ((A\rightarrow A)\rightarrow A)~~~~~~~~~~~~~~~~~~~~&A_1\\
> &\vdash (A\rightarrow ((A\rightarrow A)\rightarrow A))\rightarrow((A\rightarrow(A\rightarrow A))\rightarrow(A\rightarrow A))~~~~~~~~~~~~~~~~~~~~&A_2\\
> &\vdash (A\rightarrow(A\rightarrow A))\rightarrow(A\rightarrow A)~~~~~~~~~~~~~~~~~~~~&MP _{12}\\
> &\vdash A\rightarrow (A\rightarrow A)~~~~~~~~~~~~~~~~~~~~&A_1\\
> &\vdash A\rightarrow A~~~~~~~~~~~~~~~~~~~~&MP_{34}\\
> \end{aligned}
> $$
>

Now you can notice that we only have one kind of inference rule here in the Hilbert system, then we can tell that sometimes it is very hard to make a proof by these limited tools.

So Now we have to introduce more inference rule here.

**Rule #3**

> *Definition:*
> $$
> \vdash A \rightarrow A
> $$
> *Proof:*
> $$
> \begin{aligned}
> &\vdash A\rightarrow ((A\rightarrow A)\rightarrow A)~~~~~~~~~~~~~~~~~~~~&A_1\\
> &\vdash (A\rightarrow ((A\rightarrow A)\rightarrow A))\rightarrow((A\rightarrow(A\rightarrow A))\rightarrow(A\rightarrow A))~~~~~~~~~~~~~~~~~~~~&A_2\\
> &\vdash (A\rightarrow(A\rightarrow A))\rightarrow(A\rightarrow A)~~~~~~~~~~~~~~~~~~~~&MP _{12}\\
> &\vdash A\rightarrow (A\rightarrow A)~~~~~~~~~~~~~~~~~~~~&A_1\\
> &\vdash A\rightarrow A~~~~~~~~~~~~~~~~~~~~&MP_{34}\\
> \end{aligned}
> $$
>
> > [!NOTE]
> >
> > We can see that it is a very trivial conclusion, but it is very hard to prove it, and I think we don't need any effort to memorize this rule, but when you use it, please mention that this is a rule.

**Rule #4: Contrapositive Rule**

> *Definition:*
> $$
> \frac{\Sigma \vdash (\neg B)\rightarrow(\neg A)}{\Sigma\vdash A\rightarrow B}
> $$
> *Proof:*
> $$
> \begin{aligned}
> &\Sigma\vdash (\neg B)\rightarrow(\neg A)~~~~~~~~~~~~~~~~~~~~&Premise\\
> &\Sigma\vdash ((\neg B)\rightarrow(\neg A))\rightarrow(A\rightarrow B)~~~~~~~~~~~~~~~~~~~~&A_3\\
> &\Sigma\vdash A\rightarrow B~~~~~~~~~~~~~~~~~~~~&MP_{12}\\
> \end{aligned}
> $$
>
> > [!NOTE]
> >
> > We can see that it is telling us the relationship between the original proposition and the converse negative proposition, which the former one can imply the later one.

**Rule #5: Deduction Rule**

> **Part One**
>
> *Definition:*
> $$
> \frac{\Gamma\cup\{A\}\vdash B}{\Gamma\vdash A\rightarrow B}
> $$
> *Proof:*
>
> This can be the hardest proof in the Hilbert System.
>
> I want to separate the proposition B into all single proposition $\sum_{k=1}^{i} B_k$, and I want to use the induction rule to prove everything.
>
> When $i = 1$, then will find that there are three kinds of possibilities.
>
> 1. $B_1$ is an axiom in the Hilbert proof system.
> 2. $B_1\in \Gamma$, this is according to the $Definition_2$ of the Hilbert Proof System.
> 3. $B_1 = A$, this is also according to the $Difinition_2$ of the Hilbert Proof System.
>
> > Case One: $B_1$​ is an axiom in the Hilbert proof system.
> > $$
> > \begin{aligned}
> > &\Gamma\vdash B~~~~~~~~~~~~~~~~~~~~&Premise\\
> > &\Gamma\vdash B\rightarrow(A\rightarrow B)~~~~~~~~~~~~~~~~~~~~&A_1\\
> > &\Gamma\vdash A\rightarrow B~~~~~~~~~~~~~~~~~~~~&MP_{12}\\
> > \end{aligned}
> > $$
>
> > Case Two: $B_1\in \Gamma$
> > $$
> > \begin{aligned}
> > &\Gamma\vdash B~~~~~~~~~~~~~~~~~~~~&Premise,~Definition_2\\
> > &\Gamma\vdash B\rightarrow(A\rightarrow B)~~~~~~~~~~~~~~~~~~~~&A_1\\
> > &\Gamma\vdash A\rightarrow B~~~~~~~~~~~~~~~~~~~~&MP_{12}\\
> > \end{aligned}
> > $$
>
> > Case Three: $B_1 = A$​
> >
> > This time, it is just the same as proving $\Gamma \vdash A\rightarrow A$, and it is just the Rule #3.
>
> Then we have prove that when $i=1$, we can have $\frac{\Gamma\cup\{A\}\vdash B_i}{\Gamma\vdash A\rightarrow B_i}$
>
> But now, let us think about the situation when the value of $i$ is bigger than 1.
>
> what we want to prove now is that if we have $k<i$ that we can prove $\frac{\Gamma\cup\{A\}\vdash B_k}{\Gamma\vdash A\rightarrow B_k}$, then we can prove $\frac{\Gamma\cup\{A\}\vdash B_i}{\Gamma\vdash A\rightarrow B_i}$.
>
> I will just take $i$ to be $k+1$, when $B_i$ is $B_k\cup B_{k+1}$.
>
> Now, we will only have four possibilities.
>
> 1. $B_{k+1}$ is an axiom in the Hilbert proof system.
> 2. $B_{k+1}\in \Gamma$, this is according to the $Definition_2$ of the Hilbert Proof System.
> 3. $B_{k+1} = A$, this is also according to the $Difinition_2$​ of the Hilbert Proof System.
> 4. $B_{k+1}$ is the intermediate conclusion of the former $B_k$​ propositions.
>
> But for $B_i$, the former three conditions are very similar, so I will just take them together.
>
> > [!WARNING]
> >
> > I made some mistake here, I don't know how to prove the combination of the situations, maybe you can help me, contact me by <a href="mailto:Jingqi.SUN@outlook.com">email</a>
>
> > Case One: $B_i$​​ is an axiom in the Hilbert proof system, or $B_i\subset (\Gamma\cup A)$
> > $$
> > \begin{aligned}
> > &\Gamma\vdash B_i~~~~~~~~~~~~~~~~~~~~&Premise~or~Definition_2\\
> > &\Gamma\vdash B_i\rightarrow(A\rightarrow B_i)~~~~~~~~~~~~~~~~~~~~&A_1\\
> > &\Gamma\vdash A\rightarrow B_i~~~~~~~~~~~~~~~~~~~~&MP_{12}\\
> > \end{aligned}
> > $$
>
> > Case Two: $Bi\subset A$.
> >
> > This time, it is just the same as proving $\Gamma \vdash A\rightarrow A$, and it is just the Rule #3.
>
> > Case Three: $B_{k+1}$ is the intermediate conclusion of the former $B_k$ propositions, and I suppose those two to form the modus ponens is the $m^{th}$ and the $j^{th}$, and then we can write $B_m = B_j\rightarrow B_i$
> > $$
> > \begin{aligned}
> > &\Gamma \vdash A \rightarrow B_m~~~~~~~~~~~~~~~~~~~~&Premise\\
> > &\Gamma \vdash A \rightarrow B_j~~~~~~~~~~~~~~~~~~~~&Premise\\
> > &\Gamma \vdash A \rightarrow (B_j\rightarrow B_i)~~~~~~~~~~~~~~~~~~~~&Replacement\\
> > &\Gamma \vdash (A \rightarrow (B_j\rightarrow B_i))\rightarrow((A\rightarrow B_j)\rightarrow(A\rightarrow B_i))~~~~~~~~~~~~~~~~~~~~&A_2\\
> > &\Gamma \vdash (A\rightarrow B_j)\rightarrow(A\rightarrow B_i)~~~~~~~~~~~~~~~~~~~~&MP_{34}\\
> > &\Gamma \vdash A\rightarrow B_i~~~~~~~~~~~~~~~~~~~~&MP_{25}\\
> > \end{aligned}
> > $$
>
> So now by the definition of  the induction rule, I proved the deduction rule part one successfully.
>
> **Part Two**
>
> *Definition:*
> $$
> \frac{\Gamma\vdash A\rightarrow B}{\Gamma\cup\{A\}\vdash B}
> $$
> *Proof:*
>
> The proving method of part two is very similar to the one of part one, so that I will not show the proving progress here.

**Rule #6**

> *Definition:*
>
> $\vdash (A\rightarrow B)\rightarrow((B\rightarrow C)\rightarrow(A\rightarrow C))$
>
> *Proof:*
> $$
> \begin{aligned}
> \{(A\rightarrow B),(B\rightarrow C),A\}&\vdash A~~~~~~~~~~~~~~~~~~~~&Assumption\\
> \{(A\rightarrow B),(B\rightarrow C),A\}&\vdash (A\rightarrow B)~~~~~~~~~~~~~~~~~~~~&Assumption\\
> \{(A\rightarrow B),(B\rightarrow C),A\}&\vdash B~~~~~~~~~~~~~~~~~~~~&MP_{12}\\
> \{(A\rightarrow B),(B\rightarrow C),A\}&\vdash (B\rightarrow C)~~~~~~~~~~~~~~~~~~~~&Assumption\\
> \{(A\rightarrow B),(B\rightarrow C),A\}&\vdash C~~~~~~~~~~~~~~~~~~~~&MP_{23}\\
> \{(A\rightarrow B),(B\rightarrow C)\}&\vdash (A\rightarrow C)~~~~~~~~~~~~~~~~~~~~&Deduction_5\\
> \{(A\rightarrow B)\}&\vdash ((B\rightarrow C)\rightarrow(A\rightarrow C))~~~~~~~~~~~~~~~~~~~~&Deduction_5\\
> &\vdash (A\rightarrow B)\rightarrow((B\rightarrow C)\rightarrow(A\rightarrow C))~~~~~~~~~~~~~~~~~~~~&Deduction_5\\
> \end{aligned}
> $$
>
> > [!NOTE]
> >
> > I don't think that is a very powerful rule at least now, because we can find that the things it can do can not simplify a problem, but anyway it is still a very powerful rule.

**Rule #7: Transitivity Rule**

> *Definition:*
> $$
> \frac{\Sigma\vdash A\rightarrow B~~~~~\Sigma\vdash B\rightarrow C}{\Sigma\vdash A\rightarrow C}
> $$
> *Proof:*
> $$
> \begin{aligned}
> \{A\}\cup\Sigma&\vdash A~~~~~~~~~~~~~~~~~~~~&Assumption\\
> \{A\}\cup\Sigma&\vdash (A\rightarrow B)~~~~~~~~~~~~~~~~~~~~&Premise\\
> \{A\}\cup\Sigma&\vdash B~~~~~~~~~~~~~~~~~~~~&MP_{12}\\
> \{A\}\cup\Sigma&\vdash (B\rightarrow C)~~~~~~~~~~~~~~~~~~~~&Premise\\
> \{A\}\cup\Sigma&\vdash C~~~~~~~~~~~~~~~~~~~~&MP_{34}\\
> \Sigma&\vdash A\rightarrow C~~~~~~~~~~~~~~~~~~~~&Deduction_5\\
> \end{aligned}
> $$
>
> > [!NOTE]
> >
> > This rule is very trivial but when you want to use it, you need to give the name of it, because it doesn't appeared in the original definition of the Hilbert proof system.

**Rule #8**

> *Definition:*
> $$
> \vdash(A\rightarrow(B \rightarrow C))\rightarrow(B\rightarrow(A \rightarrow C))
> $$
> *Proof:*
> $$
> \begin{aligned}
> \{A\rightarrow(B \rightarrow C)\}&\vdash (A\rightarrow(B \rightarrow C))~~~~~~~~~~~~~~~~~~~~&Assumption\\
> \{A\rightarrow(B \rightarrow C),A\}&\vdash (B \rightarrow C)~~~~~~~~~~~~~~~~~~~~&Deduction_1\\
> \{A\rightarrow(B \rightarrow C),A,B\}&\vdash C~~~~~~~~~~~~~~~~~~~~&Deduction_2\\
> \{A\rightarrow(B \rightarrow C),B\}&\vdash (A \rightarrow C)~~~~~~~~~~~~~~~~~~~~&Deduction_3\\
> \{A\rightarrow(B \rightarrow C)\}&\vdash (B\rightarrow(A \rightarrow C))~~~~~~~~~~~~~~~~~~~~&Deduction_4\\
> &\vdash(A\rightarrow(B \rightarrow C))\rightarrow (B\rightarrow(A \rightarrow C))~~~~~~~~~~~~~~~~~~~~&Deduction_5\\
> \end{aligned}
> $$
>
> > [!NOTE]
> >
> > This is a pre-version of a very powerful rule, it can change the form of the proposition.

**Rule #9: Exchange of Antecedent Rule**

> *Definition:*
> $$
> \frac{\Sigma A\rightarrow(B \rightarrow C)}{\Sigma B\rightarrow(A\rightarrow C)}
> $$
> *Proof:*
> $$
> \begin{aligned}
> &\vdash A\rightarrow(B \rightarrow C)~~~~~~~~~~~~~~~~~~~~&Premise\\
> &\vdash(A\rightarrow(B \rightarrow C))\rightarrow (B\rightarrow(A \rightarrow C))~~~~~~~~~~~~~~~~~~~~&Rule\#8\\
> &\vdash B\rightarrow(A \rightarrow C)~~~~~~~~~~~~~~~~~~~~&MP_{12}\\
> \end{aligned}
> $$
>
> > [!NOTE]
> >
> > This is a very important rule in the Hilbert System, because it can actually help you to change the antecedent of the proposition.

**Rule #10**

> **Part One**
>
> *Definition:*
> $$
> \vdash\neg A\rightarrow(A\rightarrow B)
> $$
> *Proof:*
> $$
> \begin{aligned}
> \{\neg A\}&\vdash (\neg A)~~~~~~~~~~~~~~~~~~~~&Assumption\\
> \{\neg A\}&\vdash((\neg A)\rightarrow ((\neg B)\rightarrow(\neg A)))~~~~~~~~~~~~~~~~~~~~&A_1\\
> \{\neg A\}&\vdash ((\neg B)\rightarrow(\neg A))~~~~~~~~~~~~~~~~~~~~&MP_{12}\\
> \{\neg A\}&\vdash (A\rightarrow B)~~~~~~~~~~~~~~~~~~~~&Contrapositive_3\\
> &\vdash\neg A\rightarrow(A\rightarrow B)~~~~~~~~~~~~~~~~~~~~&Deduction_4\\
> \end{aligned}
> $$
> **Part Two**
>
> *Definition:*
> $$
> \vdash A\rightarrow(\neg A\rightarrow B)
> $$
> *Proof:*
>
> The way of proof in the part two is very similar to which of part one, so I will not do it again.
>
> > [!NOTE]
> >
> > The meaning of it is that both sides of one thing can be used to imply anything in the world, which is very easy to understand, and I think this rule is also kind of important.

**Rule #11**

> **Part One**
>
> *Definition:*
> $$
> \vdash \neg\neg A\rightarrow A
> $$
> > [!NOTE]
> >
> > I gain the idea from a webpage designed by Stanford.
>
> *Proof:*
> $$
> \begin{aligned}
> \{\neg\neg A\}&\vdash (\neg\neg A)~~~~~~~~~~~~~~~~~~~~&Assumption\\
> &\vdash (\neg\neg A)\rightarrow ((\neg\neg\neg\neg A)\rightarrow (\neg \neg A))~~~~~~~~~~~~~~~~~~~~&A_2\\
> \{\neg\neg A\}&\vdash (\neg\neg\neg\neg A)\rightarrow (\neg \neg A)~~~~~~~~~~~~~~~~~~~~&Deduction_2\\
> \{\neg\neg A\}&\vdash (\neg A)\rightarrow (\neg\neg \neg A)~~~~~~~~~~~~~~~~~~~~&Contrapositive_3\\
> \{\neg\neg A\}&\vdash (\neg\neg A)\rightarrow A~~~~~~~~~~~~~~~~~~~~&Contrapositive_4\\
> \{\neg\neg A\}&\vdash  A~~~~~~~~~~~~~~~~~~~~&MP_{15}\\
> &\vdash (\neg\neg A)\rightarrow A~~~~~~~~~~~~~~~~~~~~&Deduction_6\\
> \end{aligned}
> $$
>

> **Part Two**
>
> *Definition:*
> $$
> \vdash A\rightarrow \neg\neg A
> $$
> *Proof:*
> $$
> \begin{aligned}
> \{A\}&\vdash  A~~~~~~~~~~~~~~~~~~~~&Assumption\\
> \{A\}&\vdash  (\neg \neg \neg A)\rightarrow (\neg A)~~~~~~~~~~~~~~~~~~~~&Rule\#11PartOne\\
> \{A\}&\vdash  A\rightarrow (\neg\neg A)~~~~~~~~~~~~~~~~~~~~&Contrapositive_2\\
> &\vdash  A\rightarrow(A\rightarrow (\neg\neg A))~~~~~~~~~~~~~~~~~~~~&Deduction_3\\
> &\vdash  (A\rightarrow(A\rightarrow (\neg\neg A)))\rightarrow((A\rightarrow A)\rightarrow(A\rightarrow (\neg \neg A)))~~~~~~~~~~~~~~~~~~~~&Deduction_3\\
> &\vdash (A\rightarrow A)\rightarrow(A\rightarrow (\neg \neg A))~~~~~~~~~~~~~~~~~~~~&MP_{45}\\
> &\vdash A\rightarrow A~~~~~~~~~~~~~~~~~~~~&Rule\#3\\
> &\vdash A\rightarrow \neg \neg A~~~~~~~~~~~~~~~~~~~~&MP_{67}\\
> \end{aligned}
> $$
>
> > [!NOTE]
> >
> > This conclusion is very trivial, but the proving part is very difficult.

**Rule #12**

> **Part One**
>
> *Definition:*
> $$
> \frac{\Sigma\vdash\neg\neg A}{\Sigma\vdash A}
> $$
> *Proof:*
> $$
> \begin{aligned}
> &\vdash  \neg \neg A~~~~~~~~~~~~~~~~~~~~&Premise\\
> &\vdash  \neg \neg A\rightarrow A~~~~~~~~~~~~~~~~~~~~&Rule\#11\\
> &\vdash  A~~~~~~~~~~~~~~~~~~~~&MP_{12}\\
> \end{aligned}
> $$
> **Part Two**
>
> *Definition:*
> $$
> \frac{\Sigma\vdash A}{\Sigma\vdash \neg\neg A}
> $$
> *Proof:*
> $$
> \begin{aligned}
> &\vdash  A~~~~~~~~~~~~~~~~~~~~&Premise\\
> &\vdash  A\rightarrow \neg \neg  A~~~~~~~~~~~~~~~~~~~~&Rule\#11\\
> &\vdash  \neg \neg  A~~~~~~~~~~~~~~~~~~~~&MP_{12}\\
> \end{aligned}
> $$

**Rule #13**

> **Part One**
>
> *Definition:*
> $$
> \vdash true
> $$
> **Part Two**
>
> *Definition:*
> $$
> \vdash false
> $$
> 

> [!NOTE]
>
> Because we have proved the theorem 3, then we just find another expression that, so there is no need to prove it.

**Rule #14-1**

> *Definition:*
> $$
> \vdash (\neg A\rightarrow false)\rightarrow A
> $$
> *Proof:*
> $$
> \begin{aligned}
> \{\neg A \rightarrow false\}&\vdash (\neg A \rightarrow false)~~~~~~~~~~~~~~~~~~~~&Assumption\\
> \{\neg A \rightarrow false\}&\vdash (\neg false \rightarrow A)~~~~~~~~~~~~~~~~~~~~&Contrapositive_{1}\\
> \{\neg A \rightarrow false\}&\vdash \neg false ~~~~~~~~~~~~~~~~~~~~&Rule \#13\\
> \{\neg A \rightarrow false\}&\vdash A ~~~~~~~~~~~~~~~~~~~~&MP_{23}\\
> &\vdash (\neg A\rightarrow false)\rightarrow A ~~~~~~~~~~~~~~~~~~~~&MP_{23}\\
> \end{aligned}
> $$
>
> > [!NOTE]
> >
> > To understand this rule, if we know something that can imply the false, then we will have the opposite of this event to be true. If you think it more carefully, it is just proving by contradiction.

**Rule #14-2: Reductio ad Absurdum**

> *Definition:*
> $$
> \frac{\Sigma \vdash \neg A \rightarrow false}{\Sigma \vdash A}
> $$
> *Proof:*
> $$
> \begin{aligned}
> \Sigma &\vdash (\neg A\rightarrow false)\rightarrow A~~~~~~~~~~~~~~~~~~~~&Rule \#14-1\\
> \Sigma &\vdash \neg A \rightarrow false~~~~~~~~~~~~~~~~~~~~&Premise\\
> \Sigma &\vdash A~~~~~~~~~~~~~~~~~~~~&MP_{12}\\
> \end{aligned}\\
> $$
>
> > [!NOTE]
> >
> > This is just another form of the rule #14, you can think that if you want to form something and then some absurd contradiction forms, then you can prove the original form is true.

> [!CAUTION]
>
> **In summary, there can be statements that are provable in a Hilbert-style proof system but false in a semantic interpretation, and vice versa.** 

**Rule #15: Implication Reduction**

> *Definition:*
> $$
> \vdash (A\rightarrow \neg A)\rightarrow \neg A
> $$
> *Proof:*
> $$
> \begin{aligned}
> \{A\rightarrow \neg A,  \neg\neg A\}&\vdash \neg\neg A~~~~~~~~~~~~~~~~~~~~&Assumption\\
> \{A\rightarrow \neg A,  \neg\neg A\}&\vdash A~~~~~~~~~~~~~~~~~~~~&DoubleNegation_1\\
> \{A\rightarrow \neg A,  \neg\neg A\}&\vdash A\rightarrow \neg A~~~~~~~~~~~~~~~~~~~~&Assumption\\
> \{A\rightarrow \neg A,  \neg\neg A\}&\vdash \neg A~~~~~~~~~~~~~~~~~~~~&MP_{23}\\
> 
> \end{aligned}
> $$
> 
> 
> 

**The List Of Rule in the Hilbert Proof System**

| Sequence |          Name          |                           Content                            |
| :------: | :--------------------: | :----------------------------------------------------------: |
|    1     |       Definition       |                     Not To Mention Again                     |
|    2     |       Definition       |                     Not to Mention Again                     |
|    3     |          Null          |                   $\vdash A\rightarrow A$                    |
|    4     |     Contrapositive     | $\frac{\Sigma \vdash (\neg B)\rightarrow(\neg A)}{\Sigma\vdash A\rightarrow B}$ |
|    5     |       Deduction        | Part One: $\frac{\Gamma\cup\{A\}\vdash B}{\Gamma\vdash A\rightarrow B}$, Part Two:$\frac{\Gamma\vdash A\rightarrow B}{\Gamma\cup\{A\}\vdash B}$ |
|    6     |          Null          | $\vdash (A\rightarrow B)\rightarrow((B\rightarrow C)\rightarrow(A\rightarrow C))$ |
|    7     |      Transitivity      | $\frac{\Sigma\vdash A\rightarrow B~~~~~\Sigma\vdash B\rightarrow C}{\Sigma\vdash A\rightarrow C}$ |
|    8     |          Null          | $\vdash(A\rightarrow(B \rightarrow C))\rightarrow(B\rightarrow(A \rightarrow C))$ |
|    9     | Exchange of Antecedent | $\frac{\Sigma A\rightarrow(B \rightarrow C)}{\Sigma B\rightarrow(A\rightarrow C)}$ |
|    10    |          Null          | Part One: $\vdash\neg A\rightarrow(A\rightarrow B)$, Part Two: $\vdash A\rightarrow(\neg A\rightarrow B)$ |
|    11    |          Null          | Part One: $\vdash \neg\neg A\rightarrow A$, Part Two: $A\rightarrow \neg\neg A$ |
|    12    |    Double Negation     | Part One: $\frac{\Sigma\vdash\neg\neg A}{\Sigma\vdash A}$, Part Two: $\frac{\Sigma\vdash A}{\Sigma\vdash \neg\neg A}$ |
|    13    |          Null          |    Part One: $\vdash true$, Part Two: $\vdash \neg false$    |
|   14-1   |          Null          |       $\vdash (\neg A\rightarrow false)\rightarrow A$        |
|   14-2   |  Reductio ad Absurdum  | $\frac{\Sigma \vdash \neg A \rightarrow false}{\Sigma \vdash A}$ |
|    15    | Implication Reduction  |       $\vdash (A\rightarrow \neg A)\rightarrow \neg A$       |

**Other Resources**

https://www.youtube.com/watch?v=JhH9i47YFHQ&amp;ab_channel=WilliamSpaniel

http://logica.stanford.edu/homepage/hilbertlibrary.php

